src/coq/Semantics/Memory/MemBytes.v
@@ -52,7 +52,7 @@ Module Type ByteImpl(Addr:ADDRESS)(IP:INTPTR)(SIZEOF:Sizeof)(LLVMEvents: LLVM_IN
       sbyte_to_extractbyte (uvalue_sbyte uv dt idx sid) =  UVALUE_ExtractByte uv dt idx sid.
 End ByteImpl.
 
-Module Byte(Addr:ADDRESS)(IP:INTPTR)(SIZEOF:Sizeof)(LLVMEvents:LLVM_INTERACTIONS(Addr)(IP)(SIZEOF))(Byte:ByteImpl(Addr)(IP)(SIZEOF)(LLVMEvents)).
+Module Type ByteModule(Addr:ADDRESS)(IP:INTPTR)(SIZEOF:Sizeof)(LLVMEvents:LLVM_INTERACTIONS(Addr)(IP)(SIZEOF))(Byte:ByteImpl(Addr)(IP)(SIZEOF)(LLVMEvents)).
   Export Byte.
   Import LLVMEvents.
   Import DV.
@@ -135,4 +135,8 @@ Module Byte(Addr:ADDRESS)(IP:INTPTR)(SIZEOF:Sizeof)(LLVMEvents:LLVM_INTERACTIONS
     | UVALUE_ExtractByte uv dt idx sid => inr sid
     | _ => inl "Invalid sbyte, did not convert to extractbyte."%string
     end.
+End ByteModule.
+
+Module Byte (Addr:ADDRESS)(IP:INTPTR)(SIZEOF:Sizeof)(LLVMEvents:LLVM_INTERACTIONS(Addr)(IP)(SIZEOF))(Byte:ByteImpl(Addr)(IP)(SIZEOF)(LLVMEvents)) : ByteModule Addr IP SIZEOF LLVMEvents Byte.
+  Include (ByteModule Addr IP SIZEOF LLVMEvents Byte).
 End Byte.
